HOL-ETCS/Add.thy
@@ -579,7 +579,7 @@ proof -
   proof -
     have "add2 \<circ>\<^sub>c (id\<^sub>c \<nat>\<^sub>c \<times>\<^sub>f add2) \<circ>\<^sub>c associate_right \<nat>\<^sub>c \<nat>\<^sub>c \<nat>\<^sub>c \<circ>\<^sub>c (id\<^sub>c (\<nat>\<^sub>c \<times>\<^sub>c \<nat>\<^sub>c) \<times>\<^sub>f successor)  =
         successor \<circ>\<^sub>c add2 \<circ>\<^sub>c (id\<^sub>c \<nat>\<^sub>c \<times>\<^sub>f add2) \<circ>\<^sub>c associate_right \<nat>\<^sub>c \<nat>\<^sub>c \<nat>\<^sub>c"
-    proof (typecheck_cfuncs, rule_tac one_separator[where X="(\<nat>\<^sub>c \<times>\<^sub>c \<nat>\<^sub>c) \<times>\<^sub>c \<nat>\<^sub>c", where Y="\<nat>\<^sub>c"], clarify)
+    proof (typecheck_cfuncs, rule one_separator[where X="(\<nat>\<^sub>c \<times>\<^sub>c \<nat>\<^sub>c) \<times>\<^sub>c \<nat>\<^sub>c", where Y="\<nat>\<^sub>c"], clarify)
       fix x
       assume "x \<in>\<^sub>c (\<nat>\<^sub>c \<times>\<^sub>c \<nat>\<^sub>c) \<times>\<^sub>c \<nat>\<^sub>c"
       then obtain a b c where element_types: "a \<in>\<^sub>c \<nat>\<^sub>c" "b \<in>\<^sub>c \<nat>\<^sub>c" "c \<in>\<^sub>c \<nat>\<^sub>c" and x_def: "x = \<langle>\<langle>a,b\<rangle>,c\<rangle>"
@@ -627,7 +627,7 @@ proof -
   proof -
     have "add2 \<circ>\<^sub>c (add2 \<times>\<^sub>f id\<^sub>c \<nat>\<^sub>c) \<circ>\<^sub>c (id\<^sub>c(\<nat>\<^sub>c \<times>\<^sub>c \<nat>\<^sub>c) \<times>\<^sub>f successor)
         = successor \<circ>\<^sub>c add2 \<circ>\<^sub>c (add2 \<times>\<^sub>f id\<^sub>c \<nat>\<^sub>c)"
-    proof (typecheck_cfuncs, rule_tac one_separator[where X="(\<nat>\<^sub>c \<times>\<^sub>c \<nat>\<^sub>c) \<times>\<^sub>c \<nat>\<^sub>c", where Y="\<nat>\<^sub>c"], clarify)
+    proof (typecheck_cfuncs, rule one_separator[where X="(\<nat>\<^sub>c \<times>\<^sub>c \<nat>\<^sub>c) \<times>\<^sub>c \<nat>\<^sub>c", where Y="\<nat>\<^sub>c"], clarify)
       fix x
       assume "x \<in>\<^sub>c (\<nat>\<^sub>c \<times>\<^sub>c \<nat>\<^sub>c) \<times>\<^sub>c \<nat>\<^sub>c"
       then obtain a b c where element_types: "a \<in>\<^sub>c \<nat>\<^sub>c" "b \<in>\<^sub>c \<nat>\<^sub>c" "c \<in>\<^sub>c \<nat>\<^sub>c" and x_def: "x = \<langle>\<langle>a,b\<rangle>,c\<rangle>"
